finished proof that bind is a scott continuous function, and demonstrated scott continuity with a proof that a version of factorial written using this method is correct

theories/CPO/ITreeCPO.v
@@ -71,6 +71,13 @@ intros. econstructor. Unshelve.
   intros. inv H2. auto. eapply strong_itree_approx_trans; eauto.
 Qed.
 
+(*TODO move this to EuttDiv or something *)
+Lemma bind_spin : forall E R (k : R -> itree E R), @ITree.spin E R ≅ ITree.bind ITree.spin k.
+Proof.
+  ginit. gcofix CIH. intros. setoid_rewrite spin_cong_tau_spin.
+  rewrite bind_tau. gstep. constructor. gfinal. left. auto.
+Qed.
+
 Section Fixable.
 Context (E : Type -> Type).
 Context (taa : forall {A B C : Type} (e1 : E A) (a : A) (e2 : E B) (k : B -> C) (default : C) , C).
@@ -94,33 +101,339 @@ Proof.
     enough (strong_itree_approx eq (Tau (ITree.subst k t0) ) t ).
     + assert (paco2 (strong_itree_approx_ eq id) r (Tau (ITree.subst k t0) ) t  ). 
       eapply paco2_mon; eauto; intros; contradiction. punfold H4.
-    + rewrite H2. Admitted.
+    + rewrite H2. setoid_rewrite <- bind_spin. rewrite <- spin_cong_tau_spin.
+      apply strong_itree_approx_spin_bottom.
+Qed.
 
+(* For some reason it wasn't finding this instance so I redeclared it *)
+Instance peel_vis_elem_proper'
+     : forall R (A0 : Type) (e0 : E A0) (a0 : A0),
+       Proper (@eq_itree E R R eq ==> eq_itree eq) (peel_vis_elem taa e0 a0).
+Proof. intros. destruct Htaa. eapply peel_vis_elem_proper; eauto. Qed.
+
+Instance proper_fun_seq' R : Proper (fun_eq ==> @eq_itree E R R eq) (itree_approx_sup taa).
+Proof.
+  eapply proper_fun_seq; destruct Htaa; eauto.
+Qed.
+
+Instance proper_fun_seq_peel_vis' : forall R (A : Type) (e : E A) (a : A),
+  Proper (@fun_eq E nat R ==> fun_eq) (peel_vis taa e a).
+Proof. intros. eapply proper_fun_seq_peel_vis; destruct Htaa; auto. Qed.
+
+(* TODO move to other file *)
+Lemma weak_itree_approx_ret_spin:
+     forall (R : Type) (r : R), ~ weak_itree_approx eq (Ret r) (@ITree.spin E R).
+Proof.
+  intros R r Hcontra. punfold Hcontra. red in Hcontra.
+  cbn in *. remember (RetF r) as x. remember (TauF ITree.spin) as y.
+  hinduction Hcontra before E; intros; inv Heqx; inv Heqy; eauto.
+Qed.
+
+Lemma subst_scott_cont_aux_ret1 : forall (R : Type) (r : R) (seq : sequence (itree E R) ),
+    supremum seq (Ret r) -> ~ forall n, ~ seq n ≈ Ret r.
+Proof.
+  intros R r seq Hseq Hcontra. destruct Hseq.
+  specialize (Hlub ITree.spin).
+  assert (~ weak_itree_approx eq (Ret r) (@ITree.spin E R) ).
+  apply weak_itree_approx_ret_spin. apply H. 
+  apply Hlub. red in Hmon. cbn in *. intros n.
+  specialize (Hub n). assert (~ seq n ≈ Ret r). auto.
+  assert (seq n ≈ ITree.spin).
+  {
+    remember (seq n) as t. ginit. clear Heqt. generalize dependent t.
+    gcofix CIH. intros. punfold Hub. red in Hub.
+    cbn in *. remember (observe t) as ot. remember (RetF r) as y.
+    hinduction Hub before r; intros; inv Heqy; use_simpobs; eauto.
+    - rewrite Heqot in H1. exfalso. apply H1. reflexivity.
+    - rewrite Heqot. cbn in *. gstep. red. cbn. constructor.
+      gfinal. left. pclearbot. eapply CIH; eauto.
+      + rewrite <- itree_eta. auto.
+      + rewrite Heqot in H1. rewrite tau_eutt in H1. auto.
+  }
+  rewrite H1. apply weak_itree_approx_spin_bottom.
+Qed.
+
+Lemma subst_scott_cont_aux_ret2 : forall (R : Type) (r : R) (seq : sequence (itree E R) ),
+    supremum seq (Ret r) -> exists n, seq n ≈ Ret r.
+Proof.
+  intros. apply subst_scott_cont_aux_ret1 in H.
+  destruct (classic (exists n, seq n ≈ Ret r) ); auto.
+  exfalso. apply H. intros. intro Hcontra.
+  apply H0. exists n. eauto.
+Qed.
+
+Lemma peel_vis_supremum_eq_itree : forall (R X : Type) (seq : sequence (itree E R)) (e : E X) (k : X -> itree E R), itree_approx_sup taa seq ≅ Vis e k -> forall a, itree_approx_sup taa (peel_vis taa e a seq) ≅ (k a).
+Proof.
+  intros. 
+  destruct (observe (seq 0) ) eqn : Hseq0; symmetry in Hseq0; use_simpobs.
+  - rewrite sup_head_ret in H; eauto. pinversion H.
+  - rewrite sup_head_tau in H; eauto. pinversion H; inv CHECK.
+  - rewrite sup_head_vis in H; eauto.
+    assert (X = X0). pinversion H; inj_existT; subst; auto.
+    subst. assert (e0 = e). pinversion H; inj_existT; subst; auto.
+    subst. eapply eqit_inv_Vis in H. Unshelve. 2 : apply a. auto.
+Qed.
+
+Lemma peel_vis_supremum_aux : forall (R X : Type) (seq : sequence (itree E R)) (e : E X) (k : X -> itree E R), 
+    monotone_approx eq seq ->
+    itree_approx_sup taa seq ≈ Vis e k -> forall a, itree_approx_sup taa (peel_vis taa e a seq) ≈ (k a).
+Proof.
+  intros R X. intros seq e k Hseq H a. 
+  punfold H. red in H. cbn in *. remember (observe (itree_approx_sup taa seq) ) as x.
+  assert (go x ≅ itree_approx_sup taa seq). subst. rewrite <- itree_eta. reflexivity.
+  clear Heqx.
+  remember (VisF e k) as y.
+  hinduction H before E; intros; inv Heqy; inj_existT; subst; use_simpobs.
+  - pclearbot. rename H0 into Heqx. destruct (observe (seq 0) ) eqn : Hseq0; symmetry in Hseq0; use_simpobs.
+    + rewrite sup_head_ret in Heqx; eauto. pinversion Heqx.
+    + rewrite sup_head_tau in Heqx; eauto. pinversion Heqx; inv CHECK.
+    + rewrite sup_head_vis in Heqx; eauto.
+      assert (X = X0). pinversion Heqx; inj_existT; subst; auto.
+      subst. assert (e0 = e). pinversion Heqx; inj_existT; subst; auto.
+      subst. eapply eqit_inv_Vis in Heqx. Unshelve. 2 : apply a.
+      rewrite <- Heqx. auto.
+  - pclearbot. rename H0 into Heqx. destruct (observe (seq 0) ) eqn : Hseq0; symmetry in Hseq0; use_simpobs.
+    + rewrite sup_head_ret in Heqx; eauto. pinversion Heqx; inv CHECK0.
+    + rewrite sup_head_tau in Heqx; eauto. pinversion Heqx; try inv CHECK0. subst.
+      rewrite sup_advance_eutt. all : try (destruct Htaa; auto; fail).
+      2 : constructor; red; intros; subst; auto.
+      2 : apply peel_vis_preserves_monotone_approx; destruct Htaa; auto.
+      rewrite <- sup_peel_tau_eutt. all : try (destruct Htaa; auto; fail).
+      2 : constructor; red; intros; subst; auto.
+      2 : apply peel_vis_preserves_monotone_approx; destruct Htaa; auto; apply advance_preserves_monotone_approx; destruct Htaa; auto.
+      assert (fun_eq (peel_tau (advance (peel_vis taa e a seq))) (peel_vis taa e a (peel_tau (advance seq) ) ) ).
+      { repeat intro; subst. unfold advance, peel_tau, peel_vis.
+        specialize (@commute_peel_vis_peel_tau) as Hcom. do 2 red in Hcom.
+        unfold peel_vis, peel_tau in Hcom. rewrite Hcom; eauto. reflexivity.
+        all : destruct Htaa; auto. }
+      rewrite H0. eapply IHeqitF; eauto. apply peel_tau_preserves_monotone_approx. apply advance_preserves_monotone_approx. auto.
+      rewrite <- itree_eta. auto.
+    + rewrite sup_head_vis in Heqx; eauto. pinversion Heqx; inv CHECK0.
+Abort. (* there is some really weird problem with a failure to unify terms here, maybe I need to reduce this to a core
+             problem. I honestly have no idea if I did something wrong or if it is a bug in Coq
+             I found a way around this but wtf
+           *)
+
+Variant sup_spec {R} (sup : sequence (itree E R) -> itree E R ) : Prop :=
+  | sup_correct (Hret : forall (seq : sequence (itree E R)) r, seq 0 ≅ Ret r -> sup seq ≅ Ret r)
+                (Htau : forall seq t, seq 0 ≅ Tau t -> sup seq ≅ Tau (sup (peel_tau (advance seq))) )
+                (Hvis : forall seq  X (e : E X) k, seq 0 ≅ Vis e k -> sup seq ≅ Vis e (fun a => sup (peel_vis taa e a seq) ) )
+                (Hadv : forall seq, monotone_approx eq seq -> sup seq ≈ sup (advance seq))
+                (Hpeel_tau : forall seq, monotone_approx eq seq -> sup (peel_tau seq) ≈ sup seq  )
+                (Hprop : Proper (fun_eq ==> eq_itree eq) sup )
+.
+
+Lemma peel_vis_supremum_aux' : forall (R X : Type) (seq : sequence (itree E R)) (e : E X) (k : X -> itree E R)
+  (sup : sequence (itree E R) -> itree E R ), 
+    monotone_approx eq seq ->
+    sup_spec sup ->
+    sup seq ≈ Vis e k -> forall a, sup (peel_vis taa e a seq) ≈ (k a).
+Proof.
+  intros R X. intros seq e k sup Hseq Hsup H a. 
+  destruct Hsup. rename Hret into sup_head_ret. rename Htau into sup_head_tau.
+  rename Hvis into sup_head_vis. rename Hadv into sup_advance_eutt.
+  rename Hpeel_tau into sup_peel_tau_eutt.
+  punfold H. red in H. cbn in *. remember (observe (sup seq) ) as x.
+  assert (go x ≅ sup seq). subst. rewrite <- itree_eta. reflexivity.
+  clear Heqx.
+  remember (VisF e k) as y.
+  hinduction H before E; intros; inv Heqy; inj_existT; subst; use_simpobs.
+  - pclearbot. rename H0 into Heqx. destruct (observe (seq 0) ) eqn : Hseq0; symmetry in Hseq0; use_simpobs.
+    + rewrite sup_head_ret in Heqx; eauto. pinversion Heqx.
+    + rewrite sup_head_tau in Heqx; eauto. pinversion Heqx; inv CHECK.
+    + rewrite sup_head_vis in Heqx; eauto.
+      assert (X = X0). pinversion Heqx; inj_existT; subst; auto.
+      subst. assert (e0 = e). pinversion Heqx; inj_existT; subst; auto.
+      subst. eapply eqit_inv_Vis in Heqx. Unshelve. 2 : apply a.
+      rewrite <- Heqx. auto.
+  - pclearbot. rename H0 into Heqx. destruct (observe (seq 0) ) eqn : Hseq0; symmetry in Hseq0; use_simpobs.
+    + rewrite sup_head_ret in Heqx; eauto. pinversion Heqx; inv CHECK0.
+    + rewrite sup_head_tau in Heqx; eauto. pinversion Heqx; try inv CHECK0. subst.
+      rewrite sup_advance_eutt. 
+      2 : apply peel_vis_preserves_monotone_approx; destruct Htaa; auto.
+      rewrite <- sup_peel_tau_eutt. 
+      2 : apply peel_vis_preserves_monotone_approx; destruct Htaa; auto; apply advance_preserves_monotone_approx; destruct Htaa; auto.
+      assert (fun_eq (peel_tau (advance (peel_vis taa e a seq))) (peel_vis taa e a (peel_tau (advance seq) ) ) ).
+      { repeat intro; subst. unfold advance, peel_tau, peel_vis.
+        specialize (@commute_peel_vis_peel_tau) as Hcom. do 2 red in Hcom.
+        unfold peel_vis, peel_tau in Hcom. rewrite Hcom; eauto. reflexivity.
+        all : destruct Htaa; auto. }
+      rewrite H0. eapply IHeqitF; eauto. apply peel_tau_preserves_monotone_approx. apply advance_preserves_monotone_approx. auto.
+      rewrite <- itree_eta. auto.
+    + rewrite sup_head_vis in Heqx; eauto. pinversion Heqx; inv CHECK0. 
+Qed.
+
+Lemma peel_vis_supremum_aux : forall (R X : Type) (seq : sequence (itree E R)) (e : E X) (k : X -> itree E R), 
+    monotone_approx eq seq ->
+    itree_approx_sup taa seq ≈ Vis e k -> forall a, itree_approx_sup taa (peel_vis taa e a seq) ≈ (k a).
+Proof.
+  intros. apply peel_vis_supremum_aux'; auto. constructor.
+  - apply sup_head_ret.
+  - apply sup_head_tau.
+  - apply sup_head_vis.
+  - apply sup_advance_eutt. all : destruct Htaa; auto.
+    constructor; repeat red; intros; subst; auto.
+  - apply sup_peel_tau_eutt. all : destruct Htaa; auto.
+    constructor; repeat red; intros; subst; auto.
+  - apply proper_fun_seq'.
+Qed. 
+
+(*should be able to rely on peel_vis_supremum_aux for this, or maybe not*)
+Lemma peel_vis_supremum:
+  forall (R X : Type) (seq : sequence (itree E R)) (e : E X) (k : X -> itree E R) (a : X),
+    supremum seq (Vis e k) -> supremum (peel_vis taa e a seq) (k a).
+Proof.
+  intros R X seq e k a Hseq.
+  assert (monotone_seq seq). destruct Hseq; auto.
+  eapply CPO.sup_correct in H. 
+  assert (weak_eq (sup seq) (Vis e k)). eapply supremum_unique; eauto. apply E_itree_cpo_laws.
+  cbn in H0. eapply peel_vis_supremum_aux in H0. Unshelve. 3 : apply a.
+  2 : destruct Hseq; auto. symmetry in H0. assert (weak_eq (k a) (sup (peel_vis taa e a seq)) ).  cbn. auto. rewrite H1. apply CPO.sup_correct. red. cbn. intros.
+  apply peel_vis_preserves_monotone_approx; destruct Htaa; auto. destruct H; auto.
+Qed.
+
+Lemma supremum_to_bind_lub:
+  forall (R : Type) (k : R -> itree E R) (t : itree E R) (seq : sequence (itree E R)),
+    monotone_seq seq ->
+    (forall n : nat, weak_leq (seq n) t) ->
+    (forall upper_bound : itree E R,
+        (forall n : nat, weak_leq (seq n) upper_bound) -> weak_leq t upper_bound) ->
+    forall upper_bound : itree E R,
+      (forall n : nat, weak_itree_approx eq (map (ITree.subst k) seq n) upper_bound) ->
+      weak_itree_approx eq (ITree.subst k t) upper_bound.
+Proof.
+  intros R k t seq Hmon Hub Hlub. generalize dependent t.
+  generalize dependent seq. ginit. gcofix CIH.
+  intros seq Hmon t Hub Hlub upper_bound Hupper.
+  cbn in *. Abort.
+
+Lemma peel_vis_upper_bound_aux:
+  forall (R : Type) (k : R -> itree E R) (X : Type) (k2 : X -> itree E R)
+    (seq : sequence (itree E R)) (e0 : E X) (k0 : X -> itree E R),
+    (forall n : nat, weak_itree_approx eq (seq n) (Vis e0 k0)) ->
+    forall (a : X) (n : nat),
+      weak_itree_approx eq (map (ITree.subst k) seq n) (Vis e0 k2) ->
+      weak_itree_approx eq (map (ITree.subst k) (peel_vis taa e0 a seq) n) (k2 a).
+Proof.
+  intros R k X k2. unfold peel_vis. unfold map. intros.
+  specialize (H n) as Hn. remember (seq n) as t. clear Heqt n.
+  generalize dependent t. ginit. gcofix CIH. intros t Hek2 Ht.
+  punfold Ht. red in Ht. remember (observe t) as ot. cbn in Ht.
+  remember (VisF e0 k0) as y. hinduction Ht before r; intros; inv Heqy; inj_existT; subst; use_simpobs.
+  - rewrite Heqot. rewrite peel_vis_elem_vis_eq. 2 : destruct Htaa; auto.
+    pclearbot. rewrite Heqot in Hek2. setoid_rewrite bind_vis in Hek2.
+    pinversion Hek2; inj_existT; subst; use_simpobs.
+    gfinal. right. eapply paco2_mon; eauto; intros; contradiction.
+  - rewrite Heqot. pclearbot. rewrite peel_vis_elem_tau. setoid_rewrite bind_tau.
+    gstep. constructor. gfinal. left. eapply CIH.
+    + rewrite Heqot in Hek2. rewrite tau_eutt in Hek2. auto.
+    + rewrite <- itree_eta. auto.
+Qed.
+
+Lemma subst_scott_cont_vis_seq_aux:
+  forall (R : Type) (seq : sequence (itree E R)) (X : Type) (e : E X) (k0 : X -> itree E R),
+    supremum seq (Vis e k0) ->
+    exists (n : nat) (kn : X -> itree E R),
+      seq n ≈ Vis e kn.
+Proof.
+  intros R seq X e k0 H. 
+  enough (~ forall n kn, ~ (seq n ≈ Vis e kn)).
+  { match goal with |- ?g => destruct (classic g); auto end.
+    exfalso. apply H0. intros. intro. apply H1. eauto. }
+  intro Hcontra.
+  destruct H. cbn in *.
+  assert (forall n, seq n ≈ ITree.spin).
+  { intros. specialize (Hub n). specialize (Hcontra n).
+    remember (seq n) as t. clear Heqt. generalize dependent t.
+    ginit. gcofix CIH. intros.
+    punfold Hub. red in Hub. cbn in *. remember (observe t) as ot.
+    remember (VisF e k0) as y. hinduction Hub before r; intros; inv Heqy;
+                                 inj_existT; subst; use_simpobs.
+    + exfalso. eapply Hcontra. rewrite Heqot. reflexivity.
+    + rewrite Heqot. gstep. red. cbn. constructor. gfinal. left. eapply CIH.
+      * pclearbot. rewrite <- itree_eta. auto.
+      * intros. intro. eapply Hcontra. rewrite Heqot. rewrite tau_eutt.
+        eauto.
+  }
+  specialize (Hlub ITree.spin). setoid_rewrite H in Hlub. 
+  assert (weak_itree_approx eq (Vis e k0) ITree.spin).
+  { apply Hlub. intros. apply weak_itree_approx_refl. }
+  punfold H0. red in H0. cbn in *. remember (VisF e k0) as x.
+  remember (TauF ITree.spin) as y. 
+  hinduction H0 before R; intros; inv Heqx; inv Heqy; inj_existT; subst; eauto.
+Qed.
+
+Lemma subst_scott_cont_aux : forall (R : Type) (k : R -> itree E R) (t : itree E R) 
+                               (seq : sequence (itree E R)),
+    supremum seq t -> supremum (map (ITree.subst k) seq ) (ITree.subst k t).
+Proof.
+  intros. destruct H. constructor; cbn.
+  - red. cbn. intros. apply subst_mon. auto.
+  - intros. unfold map. eapply weak_itree_approx_bind; cbn in *; eauto.
+    intros; subst. apply weak_itree_approx_refl.
+  - cbn in *. intros. generalize dependent t. generalize dependent seq. revert upper_bound.
+    ginit. gcofix CIH. intros.
+    destruct (observe t) eqn : Ht; symmetry in Ht; use_simpobs.
+    + rewrite Ht. setoid_rewrite bind_ret_l.
+      setoid_rewrite Ht in Hub.
+      unfold map in H0. setoid_rewrite Ht in Hlub.
+      clear CIH. enough (weak_itree_approx eq (k r0) upper_bound ).
+      { gfinal. right. eapply paco2_mon; eauto; intros; contradiction. }
+      assert (supremum seq (Ret r0) ). constructor; eauto.
+      apply subst_scott_cont_aux_ret2 in H. destruct H as [n Hn].
+      specialize (H0 n). rewrite Hn in H0. setoid_rewrite bind_ret_l in H0. auto.
+    + rewrite Ht. setoid_rewrite bind_tau. gstep. constructor.
+      gfinal. left. eapply CIH; eauto.
+      * setoid_rewrite Ht in Hub. setoid_rewrite tau_eutt in Hub. auto.
+      * intros. setoid_rewrite Ht in Hlub. setoid_rewrite tau_eutt in Hlub.
+        eauto.
+    + rewrite Ht. setoid_rewrite bind_vis.
+      (* from here I show that all seq n must be eutt to Vis e k with some properties on k
+         then can rewrite that into H and induct to show that upperbound must have some e
+         actually there is a complication because I know there exists some n where seq n has that prop 
+         (actually infinitely many but one is all I need)
+       *)
+      assert (exists (n : nat), exists kn, seq n ≈ Vis e kn /\ (forall a, weak_itree_approx eq (kn a) (k0 a) )  ).
+      assert (supremum seq (Vis e k0)).
+      setoid_rewrite Ht in Hub. setoid_rewrite Ht in Hlub. constructor; auto.
+      apply subst_scott_cont_vis_seq_aux in H.
+      decompose record H. eexists. eexists. split; eauto.
+      specialize (Hub x). rewrite H2 in Hub. rewrite Ht in Hub.
+      pinversion Hub. inj_existT. subst. auto.
+      decompose record H. rename x0 into kn. specialize (H0 x) as Hx.
+      unfold map in Hx. rewrite H1 in Hx. setoid_rewrite bind_vis in Hx.
+      punfold Hx. red in Hx. cbn in *. remember (VisF e (fun x : X => ITree.bind (kn x) k)) as y.
+      remember (observe upper_bound) as oub. hinduction Hx before r; intros;
+                                               inv Heqy; inj_existT; use_simpobs; subst.
+      * rewrite Heqoub. gstep. constructor. gfinal. pclearbot. left. 
+        eapply CIH with (seq := peel_vis taa e0 a seq); eauto.
+        -- apply peel_vis_preserves_monotone_approx; destruct Htaa; eauto.
+        -- setoid_rewrite Heqoub in H0. rename H0 into Hseq.
+           intros n. 
+           specialize (Hseq n) as Hseqn. 
+           setoid_rewrite Ht in Hub. eapply peel_vis_upper_bound_aux; eauto.
+        -- intros. 
+           assert (supremum seq (Vis e0 k0)).
+           setoid_rewrite Ht in Hub. setoid_rewrite Ht in Hlub. constructor; auto.
+           eapply peel_vis_supremum in H4. destruct H4; cbn in *; eauto.
+        -- intros. 
+           setoid_rewrite Ht in Hlub.
+           assert (supremum seq (Vis e0 k0) ).
+           constructor; auto. setoid_rewrite <- Ht. auto.
+           assert (supremum (peel_vis taa e0 a seq) (k0 a) ).
+           apply peel_vis_supremum; auto.
+           destruct H6. eapply Hlub0. apply H4.
+      * rewrite Heqoub. rewrite tau_euttge. eapply IHHx; eauto.
+        setoid_rewrite Heqoub in H0. setoid_rewrite tau_eutt in H0. auto.
+Qed.
 
 Lemma subst_scott_cont R (k : R -> itree E R) : scott_continuous (ITree.subst k).
 Proof.
-  red. cbn. unfold monotone_seq. cbn. ginit. gcofix CIH. intros seq Hmon.
-  assert (strong_itree_approx eq (seq 0) (seq 1) ). auto.
-  pinversion H; use_simpobs.
-  - unfold map. rewrite sup_head_ret; eauto. setoid_rewrite bind_ret_l.
-    subst.
-    (* from here I can prove that seq n ≅ k r2 forall n, then can prove that the sup of a constant seq is the constant 
-       val, then I am done, will require more meta theory, but nothing I haven't already though of*)
-    admit.
-  - unfold map. rewrite sup_head_vis; eauto. setoid_rewrite bind_vis.
-    setoid_rewrite sup_head_vis. 2 : rewrite H0; setoid_rewrite bind_vis; reflexivity.
-    gstep. constructor. 
-    unfold ITree.bind. (*if I can commute peel vis with map ITree.subst then this should work out fine *)
-    admit.
-    (* gfinal. left. eapply CIH. *)
-  - unfold map. rewrite sup_head_tau; eauto. setoid_rewrite bind_tau.
-    setoid_rewrite sup_head_tau at 2.
-    2 : { rewrite H0. setoid_rewrite bind_tau. reflexivity. }
-    unfold ITree.bind. gstep. constructor. (*again need to move map ITree.subst to the front *) admit.
-  - unfold map. rewrite sup_head_tau; eauto. setoid_rewrite bind_tau.
-    setoid_rewrite sup_head_tau at 2.
-    2 : { rewrite H0. setoid_rewrite bind_tau. reflexivity. }
-    gstep. constructor. (*one again same *) admit.
-Admitted.
+  red. intros seq Hmon. eapply CPO.sup_correct in Hmon as Hsup.
+  eapply subst_scott_cont_aux in Hsup. Unshelve. all : auto.
+  eapply supremum_unique; eauto. apply itree_weak_cpo_laws; auto.
+  apply CPO.sup_correct. red. cbn. intros.
+  cbn. unfold map. eapply subst_mon. auto.
+Qed.
 
 End Fixable.
